DecompositionOne proved; now applying it to the fifo refinement proof

src/DecompositionOne.v
@@ -10,7 +10,6 @@ Section Decomposition.
 
   Variable specRegName: string.
   Variable eta: RegsT -> option (sigT (fullType type)).
-
   Definition theta (r: RegsT): RegsT :=
     match eta r with
     | Some er => M.add specRegName er (M.empty _)
@@ -24,15 +23,19 @@ Section Decomposition.
   Hypothesis HdefSubset: forall f, In f (getDefs spec) -> In f (getDefs imp).
   Hypothesis HcallSubset: forall f, In f (getCalls spec) -> In f (getCalls imp).
 
+  Definition ConsistentUpdate (oImp oSpec: RegsT) (uImp uSpec: UpdatesT) :=
+    (uImp = M.empty _ -> uSpec = M.empty _) /\
+    (uSpec = M.empty _ -> uImp = M.empty _) /\
+    M.union uSpec (theta oImp) = theta (M.union uImp oImp).
+
   Hypothesis HsubstepRuleMap:
     forall oImp uImp rule csImp,
       reachable oImp imp ->
       Substep imp oImp uImp (Rle (Some rule)) csImp ->
       exists uSpec,
         Substep spec (theta oImp) uSpec (Rle (ruleMap oImp rule)) (liftToMap1 p csImp) /\
-        (* M.find specRegName uSpec <> M.find specRegName (theta oImp) /\ *)
-        M.union uSpec (theta oImp) = theta (M.union uImp oImp).
-
+        ConsistentUpdate oImp (theta oImp) uImp uSpec.
+  
   Definition liftP meth :=
     match meth with
     | (n :: t)%struct => match p n t with
@@ -47,10 +50,9 @@ Section Decomposition.
       Substep imp oImp uImp (Meth (Some meth)) csImp ->
       exists uSpec,
         Substep spec (theta oImp) uSpec (Meth (liftP meth)) (liftToMap1 p csImp) /\
-        (* M.find specRegName uSpec <> M.find specRegName (theta oImp) /\ *)
-        M.union uSpec (theta oImp) = theta (M.union uImp oImp).
+        ConsistentUpdate oImp (theta oImp) uImp uSpec.
 
-  Definition liftUnitLabel o ul :=
+  Definition mapUnitLabel o ul :=
     match ul with
     | Rle (Some r) => Rle (ruleMap o r)
     | Rle None => Rle None
@@ -58,117 +60,263 @@ Section Decomposition.
     | Meth None => Meth None
     end.
 
+  Lemma substepMap:
+    forall oi ui uli csi,
+      reachable oi imp ->
+      Substep imp oi ui uli csi ->
+      exists us,
+        Substep spec (theta oi) us (mapUnitLabel oi uli) (liftToMap1 p csi) /\
+        ConsistentUpdate oi (theta oi) ui us.
+  Proof.
+    intros; destruct uli as [[r|]|[dm|]].
+
+    - apply HsubstepRuleMap; auto.
+    - inv H0; exists (M.empty _); split.
+      + apply EmptyRule.
+      + unfold ConsistentUpdate; repeat split; auto.
+    - apply HsubstepMethMap; auto.
+    - inv H0; exists (M.empty _); split.
+      + apply EmptyMeth.
+      + unfold ConsistentUpdate; repeat split; auto.
+  Qed.
+
+  Record SubstepRel oImp :=
+    { uImp: UpdatesT;
+      ulImp: UnitLabel;
+      csImp: MethsT;
+      HssImp: Substep imp oImp uImp ulImp csImp;
+      uSpec: UpdatesT;
+      HssSpec: Substep spec (theta oImp) uSpec
+                       (mapUnitLabel oImp ulImp) (liftToMap1 p csImp);
+      Hcu: ConsistentUpdate oImp (theta oImp) uImp uSpec
+    }.
+
+  Definition toSubstepRecImp {oImp} (sr: SubstepRel oImp) :=
+    {| upd := uImp sr;
+       unitAnnot := ulImp sr;
+       cms := csImp sr;
+       substep := HssImp sr
+    |}.
+
+  Definition toSubstepRecSpec {oImp} (sr: SubstepRel oImp) :=
+    {| upd := uSpec sr;
+       unitAnnot := mapUnitLabel oImp (ulImp sr);
+       cms := liftToMap1 p (csImp sr);
+       substep := HssSpec sr
+    |}.
+
+  Inductive SubstepRels {oImp}: list (SubstepRel oImp) -> Prop :=
+  | SubstepMapNil: SubstepRels nil
+  | SubstepMapCons:
+      forall srs sr,
+        SubstepRels srs ->
+        (forall sr', In sr' srs -> canCombine (toSubstepRecImp sr)
+                                              (toSubstepRecImp sr')) ->
+        SubstepRels (sr :: srs).
+
   Hypothesis HcanCombine:
     forall oi ui1 ui2 uli1 uli2 csi1 csi2,
       reachable oi imp ->
       Substep imp oi ui1 uli1 csi1 ->
       Substep imp oi ui2 uli2 csi2 ->
       CanCombineUL ui1 ui2 (getLabel uli1 csi1) (getLabel uli2 csi2) ->
-      forall os us1 us2 uls1 uls2 css1 css2,
-        os = theta oi ->
-        uls1 = liftUnitLabel oi uli1 ->
-        uls2 = liftUnitLabel oi uli2 ->
-        Substep spec os us1 uls1 css1 ->
-        Substep spec os us2 uls2 css2 ->
-        M.union us1 os = theta (M.union ui1 oi) ->
-        M.union us2 os = theta (M.union ui2 oi) ->
-        CanCombineUL us1 us2 (getLabel uls1 css1) (getLabel uls2 css2).
+      forall us1 us2 css1 css2,
+        Substep spec (theta oi) us1 (mapUnitLabel oi uli1) css1 ->
+        Substep spec (theta oi) us2 (mapUnitLabel oi uli2) css2 ->
+        CanCombineUL us1 us2
+                     (getLabel (mapUnitLabel oi uli1) css1)
+                     (getLabel (mapUnitLabel oi uli2) css2).
 
-  Lemma canCombine_substepsInd:
-    forall oi ui1 ui2 li1 uli2 csi2,
-      reachable oi imp ->
-      SubstepsInd imp oi ui1 li1 ->
-      Substep imp oi ui2 uli2 csi2 ->
-      CanCombineUUL ui1 li1 ui2 csi2 uli2 ->
-      forall os us1 us2 ls1 uls2 css2,
-        os = theta oi ->
-        ls1 = liftPLabel (liftToMap1 p) ruleMap oi li1 ->
-        uls2 = liftUnitLabel oi uli2 ->
-        SubstepsInd spec os us1 ls1 ->
-        Substep spec os us2 uls2 css2 ->
-        M.union us1 os = theta (M.union ui1 oi) ->
-        M.union us2 os = theta (M.union ui2 oi) ->
-        CanCombineUUL us1 ls1 us2 css2 uls2.
+  Lemma substeps_substepRels_imp:
+    forall {oImp} (Hreach: reachable oImp imp)
+           (ss: Substeps imp oImp) (Hcomb: substepsComb ss),
+    exists (srs: list (SubstepRel oImp)),
+      map toSubstepRecImp srs = ss /\ SubstepRels srs.
   Proof.
-    induction 2; simpl; intros; subst.
-    
-    - admit.
-      
-    - specialize (IHSubstepsInd H5).
-      assert (CanCombineUUL u l ui2 csi2 uli2).
-      { eapply unionCanCombineUUL.
-        instantiate (1:= {| substep:= H1 |}); auto.
-      }
-      specialize (IHSubstepsInd H3); clear H3.
-      admit.
+    induction ss; simpl; intros; [exists nil; split; auto; constructor|].
+    inv Hcomb; specialize (IHss H1).
+    destruct IHss as [psrs ?]; dest.
+    destruct a as [su sul scs Hss].
+    destruct (substepMap Hreach Hss) as [sus ?]; dest.
+    exists ({| HssImp := Hss; HssSpec := H3; Hcu:= H4 |} :: psrs); split.
+    - simpl; f_equal; auto.
+    - constructor; auto.
+      unfold toSubstepRecImp; simpl.
+      clear -H2 H.
+      intros; apply in_map with (f:= toSubstepRecImp) in H0.
+      rewrite H in H0; auto.
   Qed.
 
-  Lemma decomposition_substepsInd:
-    forall oImp uImp lImp,
-      reachable oImp imp ->
-      SubstepsInd imp oImp uImp lImp ->
-      exists uSpec,
-        SubstepsInd spec (theta oImp) uSpec (liftPLabel (liftToMap1 p) ruleMap oImp lImp) /\
-        M.union uSpec (theta oImp) = theta (M.union uImp oImp).
+  Lemma substepRels_canCombine:
+    forall {oi} (Hreach: reachable oi imp)
+           (srs: list (SubstepRel oi))
+           sui suli scsi sus Hssi Hsss
+           (Hcombi : forall sr' : SubstepRel oi,
+               In sr' srs ->
+               canCombine {| upd := sui; unitAnnot := suli; cms := scsi; substep := Hssi |}
+                          {| upd := uImp sr'; unitAnnot := ulImp sr'; cms := csImp sr';
+                             substep := HssImp sr' |}),
+    forall s': SubstepRec spec (theta oi),
+      In s' (map toSubstepRecSpec srs) ->
+      canCombine
+        {| upd := sus;
+           unitAnnot := mapUnitLabel oi suli;
+           cms := liftToMap1 p scsi;
+           substep := Hsss |} s'.
   Proof.
-    induction 2; [exists (M.empty _); split; [constructor|auto]|subst].
+    intros.
+    apply in_map_iff in H.
+    destruct H as [nsr ?]; dest; subst.
+    specialize (Hcombi _ H0); clear H0.
+    destruct nsr as [nui nuli ncsi Hnssi nus ncss Hnsss]; simpl in *.
+    unfold toSubstepRecSpec; simpl.
 
-    destruct sul as [[r|]|[dm|]].
+    apply canCombine_CanCombineUL.
+    apply canCombine_CanCombineUL in Hcombi.
+    eapply HcanCombine; eauto.
+  Qed.
 
-    - destruct IHSubstepsInd as [uspecs ?]; dest.
-      destruct (HsubstepRuleMap H H1) as [uspec ?]; dest.
-      exists (M.union uspecs uspec); split.
-      + eapply SubstepsCons; eauto.
-        * eapply canCombine_substepsInd; eauto.
-        * unfold liftPLabel; destruct l as [a d c]; simpl; f_equal.
-          { destruct a as [[|]|]; auto. }
-          { inv H2; dest; simpl in *.
-            apply liftToMap1_union; auto.
-          }
-      + admit. (* update consistency by singleton property *)
+  Lemma substepRels_substeps_spec:
+    forall {oi} (Hreach: reachable oi imp)
+           (srs: list (SubstepRel oi)),
+      SubstepRels srs ->
+      exists (ss: Substeps spec (theta oi)),
+        map toSubstepRecSpec srs = ss /\ substepsComb ss.
+  Proof.
+    induction srs; simpl; intros; [exists nil; split; auto; constructor|].
+    inv H; specialize (IHsrs H2).
+    destruct IHsrs as [pss ?]; dest.
+    destruct a as [sui suli scsi Hssi sus Hsss].
+    exists ({| substep := Hsss |} :: pss); split.
+    - simpl; f_equal; auto.
+    - constructor; auto.
+      subst; unfold toSubstepRecImp in H3; simpl in H3.
 
-    - destruct IHSubstepsInd as [uspecs ?]; dest.
-      inv H1.
-      exists uspecs; split.
-      + eapply SubstepsCons.
-        * exact H3.
-        * apply EmptyRule.
-        * clear -H2; inv H2; dest.
-          repeat split; auto.
-          destruct l as [[[|]|] d c]; simpl in *; auto.
-        * auto.
-        * unfold liftPLabel; destruct l as [a d c]; simpl; f_equal.
-          destruct a as [[|]|]; auto.
-      + mred.
+      clear -H3 Hreach HcanCombine.
+      eapply substepRels_canCombine; eauto.
+  Qed.
 
-    - destruct IHSubstepsInd as [uspecs ?]; dest.
-      destruct (HsubstepMethMap H H1) as [uspec ?]; dest.
-      exists (M.union uspecs uspec); split.
-      + eapply SubstepsCons; eauto.
-        * eapply canCombine_substepsInd; eauto.
-        * inv H2; dest.
-          destruct l as [a d c]; simpl in *; f_equal.
-          { rewrite liftToMap1_union.
-            { f_equal.
-              destruct dm as [dmn dmb]; simpl.
-              rewrite liftToMap1AddOne.
-              destruct (p dmn dmb); auto.
-            }
-            { destruct dm as [dmn dmb]; simpl.
-              apply M.Disj_add_1; auto.
-              destruct a; auto.
-            }
-          }
-          { apply liftToMap1_union; auto. }
-      + admit. (* update consistency *)
+  Lemma liftPLabel_mergeLabel:
+    forall o l1 l2,
+      CanCombineLabel l1 l2 ->
+      liftPLabel (liftToMap1 p) ruleMap o (mergeLabel l1 l2) =
+      mergeLabel (liftPLabel (liftToMap1 p) ruleMap o l1)
+                 (liftPLabel (liftToMap1 p) ruleMap o l2).
+  Proof.
+    intros; destruct l1 as [a1 d1 c1], l2 as [a2 d2 c2]; simpl in *; f_equal.
 
-    - destruct IHSubstepsInd as [uspecs ?]; dest.
-      inv H1.
-      exists uspecs; split.
-      + p_equal H3; f_equal.
-        destruct l as [a d c]; auto.
-      + mred.
+    - destruct a1 as [[|]|], a2 as [[|]|]; reflexivity.
+    - inv H; dest; simpl in *.
+      apply liftToMap1_union; auto.
+    - inv H; dest; simpl in *.
+      apply liftToMap1_union; auto.
+  Qed.
 
+  Lemma liftPLabel_substepRels:
+    forall {oi} (srs: list (SubstepRel oi)),
+      SubstepRels srs ->
+      liftPLabel (liftToMap1 p) ruleMap oi (foldSSLabel (map toSubstepRecImp srs)) =
+      foldSSLabel (map toSubstepRecSpec srs).
+  Proof.
+    induction srs; simpl; intros; [reflexivity|].
+    inv H. specialize (IHsrs H2).
+    rewrite <-IHsrs; clear IHsrs H2.
+    unfold addLabelLeft; rewrite liftPLabel_mergeLabel.
+    f_equal.
+    - destruct a as [ui uli csi Hssi us Hsss Hcuis].
+      unfold toSubstepRecImp, toSubstepRecSpec in *; simpl in *.
+      unfold getSLabel, getLabel; f_equal; simpl; auto.
+      + destruct uli as [[|]|[|]]; auto.
+      + unfold mapUnitLabel, liftP.
+        destruct uli as [[|]|[|]]; auto.
+        destruct a as [an ab]; simpl.
+        rewrite liftToMap1AddOne.
+        destruct (p an ab); auto.
+      
+    - assert (forall ss: SubstepRec imp oi,
+                 In ss (map toSubstepRecImp srs) -> canCombine (toSubstepRecImp a) ss).
+      { intros; apply in_map_iff in H; dest; subst; auto. }
+      clear H3.
+      apply canCombine_consistent_1 in H; clear -H.
+      generalize dependent (foldSSLabel (map toSubstepRecImp srs)); intros.
+      inv H; dest; clear H0.
+      repeat split; auto.
+      + destruct a; simpl in *.
+        destruct ulImp0 as [|[|]]; auto.
+        destruct a as [an ab]; simpl in *.
+        destruct (annot l); auto.
+      + destruct a; simpl in *.
+        destruct ulImp0 as [|[|]]; auto.
+  Qed.
+
+  Lemma consistentUpdate_update_spec:
+    forall (oi os: RegsT) (ui us: UpdatesT),
+      ConsistentUpdate oi os ui us ->
+      us = M.empty _ \/ exists v, us = M.add specRegName v (M.empty _).
+  Proof.
+    intros; inv H; dest.
+    remember (M.find specRegName us) as uv; destruct uv.
+
+    - right; exists s; meq.
+      assert (M.find y (M.union us (theta oi)) =
+              M.find y (theta (M.union ui oi))) by (rewrite H1; reflexivity).
+      unfold theta in H2; destruct (eta (M.union ui oi)); findeq.
+
+    - left; meq.
+      exfalso; M.cmp y specRegName.
+      + findeq.
+      + assert (M.find y (M.union us (theta oi)) =
+                M.find y (theta (M.union ui oi))) by (rewrite H1; reflexivity).
+        unfold theta in H2; destruct (eta (M.union ui oi)); findeq.
+  Qed.
+
+  Lemma substepRels_consistentUpdate:
+    forall oi,
+      reachable oi imp ->
+      forall (srs: list (SubstepRel oi)),
+        SubstepRels srs ->
+        ConsistentUpdate oi (theta oi) (foldSSUpds (map toSubstepRecImp srs))
+                         (foldSSUpds (map toSubstepRecSpec srs)).
+  Proof.
+    induction 2; simpl; intros;
+      [unfold ConsistentUpdate; repeat split; auto|].
+
+    pose proof (consistentUpdate_update_spec IHSubstepRels).
+    unfold ConsistentUpdate in *; dest; repeat split.
+    - intros.
+      destruct sr as [ui uli csi Hssi us Hsss [? [? ?]]]; simpl in *.
+      apply M.union_empty in H6; dest.
+      unfold toSubstepRecImp in H1; simpl in H1; subst.
+      specialize (e eq_refl); subst.
+      mred.
+    - intros.
+      destruct sr as [ui uli csi Hssi us Hsss [? [? ?]]]; simpl in *.
+      apply M.union_empty in H6; dest.
+      unfold toSubstepRecImp in H1; simpl in H1; subst.
+      specialize (e0 eq_refl); subst.
+      mred.
+    - destruct H2.
+      + rewrite H2 in *.
+        specialize (H4 eq_refl); rewrite H4 in *.
+        mred.
+        clear; destruct sr; simpl in *.
+        inv Hcu0; dest; auto.
+      + destruct sr as [ui uli csi Hssi us Hsss Hcuis]; simpl in *.
+        pose proof (consistentUpdate_update_spec Hcuis).
+        unfold toSubstepRecImp in H1; simpl in H1.
+        inv Hcuis; dest.
+        destruct H6.
+
+        * subst.
+          specialize (H8 eq_refl); subst.
+          mred.
+        * exfalso.
+          pose proof (substepRels_canCombine (sui:= ui) (Hssi:= Hssi) H srs Hsss H1).
+          apply canCombine_consistent_1 in H10.
+          dest; subst.
+          rewrite H2 in H10; clear -H10.
+          inv H10; dest; clear -H.
+          specialize (H specRegName); destruct H; findeq.
   Qed.
 
   Lemma liftPLabel_hide:
@@ -215,37 +363,45 @@ Section Decomposition.
       rewrite liftToMap1_find, H0; auto.
   Qed.
 
-  Lemma liftPLabel_hide_wellHidden:
-    forall o l,
-      M.KeysSubset (defs l) (getDefs imp) ->
-      M.KeysSubset (calls l) (getCalls imp) ->
-      wellHidden imp (hide l) ->
-      wellHidden spec (hide (liftPLabel (liftToMap1 p) ruleMap o l)).
+  Lemma substepRels_wellHidden:
+    forall o,
+      reachable o imp ->
+      forall (srs: list (SubstepRel o)),
+        SubstepRels srs ->
+        wellHidden imp (hide (foldSSLabel (map toSubstepRecImp srs))) ->
+        wellHidden spec (hide (foldSSLabel (map toSubstepRecSpec srs))).
   Proof.
-    intros; rewrite <-liftPLabel_hide; auto.
-    apply liftPLabel_wellHidden; auto.
+    intros.
+    pose proof (liftPLabel_wellHidden o H1).
+    rewrite liftPLabel_hide in H2; auto.
+    - rewrite liftPLabel_substepRels in H2; auto.
+    - unfold M.KeysSubset; apply staticDynDefsSubsteps.
+    - unfold M.KeysSubset; apply staticDynCallsSubsteps; auto.
   Qed.
-    
-  Theorem decomposition_singleton:
+
+  Theorem decompositionOne:
     traceRefines (liftToMap1 p) imp spec.
   Proof.
     apply stepRefinement with (theta:= theta) (ruleMap:= ruleMap); auto.
     intros.
 
-    apply step_consistent in H0; inv H0.
-    pose proof (decomposition_substepsInd H HSubSteps) as Hdecompose.
-    destruct Hdecompose as [uspec ?]; dest.
-    exists uspec; split; auto.
+    inv H0.
+    apply substeps_substepRels_imp in HSubsteps; auto.
+    destruct HSubsteps as [srs ?]; dest.
+    pose proof (substepRels_consistentUpdate H H1).
+    pose proof (substepRels_substeps_spec H H1).
+    destruct H3 as [sss ?]; dest.
+    exists (foldSSUpds sss); split.
 
-    apply step_consistent.
-    rewrite liftPLabel_hide; auto.
-    - constructor; auto.
-      apply liftPLabel_hide_wellHidden; auto.
-      + eapply substepsInd_defs_in; eauto.
-      + eapply substepsInd_calls_in; eauto.
-    - eapply substepsInd_defs_in; eauto.
-    - eapply substepsInd_calls_in; eauto.
+    - rewrite liftPLabel_hide; auto.
+      + subst; rewrite liftPLabel_substepRels; auto.
+        constructor; auto.
+        apply substepRels_wellHidden; auto.
+      + unfold M.KeysSubset; apply staticDynDefsSubsteps.
+      + unfold M.KeysSubset; apply staticDynCallsSubsteps; auto.
+
+    - subst; unfold ConsistentUpdate in H2; dest; auto.
   Qed.
-  
+      
 End Decomposition.
 
