examples/FifoCorrect.v
@@ -1,0 +1,148 @@
+Require Import Arith.Peano_dec Bool String List.
+Require Import Lib.CommonTactics Lib.ilist Lib.Word Lib.Struct.
+Require Import Lib.FMap Lib.Indexer Lib.StringBound.
+Require Import Syntax Semantics SemFacts Equiv Refinement Tactics DecompositionOne.
+Require Import Ex.Fifo Ex.NativeFifo.
+
+Section Facts.
+  Variable fifoName: string.
+  Variable sz: nat.
+  Variable dType: Kind.
+  Variable default: ConstT dType.
+
+  Definition fifo := fifo fifoName sz dType.
+  Definition nfifo := @nativeFifo fifoName dType default.
+  Hint Unfold fifo nfifo: ModuleDefs.
+
+  Notation "^ s" := (fifoName .. s) (at level 0).
+
+  Fixpoint fifo_nfifo_elt_not_full
+           (eltv : word sz -> type dType)
+           (enqPv : word sz)
+           (edSub : nat): list (type dType) :=
+    match edSub with
+    | O => nil
+    | S ed =>
+      (eltv (enqPv ^- (natToWord sz edSub)))
+        :: (fifo_nfifo_elt_not_full eltv enqPv ed)
+    end.
+
+  Definition fifo_nfifo_eta (r: RegsT): option (sigT (fullType type)).
+  Proof.
+    kgetv ^"elt"%string eltv r (Vector dType sz) (None (A:= sigT (fullType type))).
+    kgetv ^"empty"%string emptyv r Bool (None (A:= sigT (fullType type))).
+    kgetv ^"full"%string fullv r Bool (None (A:= sigT (fullType type))).
+    kgetv ^"enqP"%string enqPv r (Bit sz) (None (A:= sigT (fullType type))).
+    kgetv ^"deqP"%string deqPv r (Bit sz) (None (A:= sigT (fullType type))).
+
+    refine (Some (existT _ (listEltK dType type) _)).
+    destruct (weq enqPv deqPv).
+    - refine (if fullv then _ else _).
+      + exact ((eltv deqPv) :: (fifo_nfifo_elt_not_full eltv enqPv (wordToNat (wones sz)))).
+      + exact nil.
+    - exact (fifo_nfifo_elt_not_full eltv enqPv (wordToNat (enqPv ^- deqPv))).
+  Defined.
+  Hint Unfold fifo_nfifo_eta: MethDefs.
+
+  Definition fifo_nfifo_theta (r: RegsT): RegsT :=
+    match fifo_nfifo_eta r with
+    | Some er => M.add ^"elt" er (M.empty _)
+    | None => M.empty _
+    end.
+  Hint Unfold fifo_nfifo_theta: MethDefs.
+  
+  Definition fifo_nfifo_ruleMap (_: RegsT) (r: string): option string := Some r.
+  Hint Unfold fifo_nfifo_ruleMap: MethDefs.
+
+  Definition fifo_inv_0 (o: RegsT): Prop.
+  Proof.
+    kexistv ^"elt"%string eltv o (Vector dType sz).
+    kexistv ^"empty"%string emptyv o Bool.
+    kexistv ^"full"%string fullv o Bool.
+    kexistv ^"enqP"%string enqPv o (Bit sz).
+    kexistv ^"deqP"%string deqPv o (Bit sz).
+    exact True.
+  Defined.
+  Hint Unfold fifo_inv_0: InvDefs.
+
+  Lemma fifo_inv_0_ok':
+    forall init n ll,
+      init = initRegs (getRegInits fifo) ->
+      Multistep fifo init n ll ->
+      fifo_inv_0 n.
+  Proof.
+    induction 2.
+
+    - simpl in H; kinv_magic.
+
+    - specialize (IHMultistep H); subst; clear H0.
+      apply step_consistent in HStep; inv HStep.
+
+      clear HWellHidden; induction HSubSteps; [auto|subst].
+      inv H; [mred|mred|inv HInRules|].
+
+      inv H0.
+      rewrite M.union_comm with (m1:= u) by auto.
+      rewrite <-M.union_assoc.
+      generalize dependent (M.union u n); intros.
+
+      clear H H1.
+      CommonTactics.dest_in; simpl in *; invertActionRep.
+
+      + kinv_magic.
+      + kinv_magic.
+      + kinv_magic.
+  Qed.
+
+  Lemma fifo_inv_0_ok:
+    forall o,
+      reachable o fifo ->
+      fifo_inv_0 o.
+  Proof.
+    intros; inv H; inv H0.
+    eapply fifo_inv_0_ok'; eauto.
+  Qed.
+
+  Lemma fifo_refines_nativefifo: fifo <<== nfifo.
+  Proof.
+    admit.
+    (* apply decompositionOne with (eta:= fifo_nfifo_eta) *)
+    (*                               (ruleMap:= fifo_nfifo_ruleMap) *)
+    (*                               (specRegName:= ^"elt"); *)
+    (*   [unfold theta; kdecompose_regmap_init; kinv_finish| | | | | |]. *)
+
+    (* - kequiv. *)
+    (* - unfold theta; kdecompose_regmap_init; kinv_finish. *)
+    (* - auto. *)
+    (* - auto. *)
+    (* - intros; inv H0; inv HInRules. *)
+    (* - intros; inv H0. *)
+    (*   CommonTactics.dest_in; simpl in *; invertActionRep. *)
+    (*   + admit. *)
+    (*   + admit. *)
+    (*   + admit. *)
+
+    (* - intros; subst. *)
+    (*   inv H0; inv H1; inv H3; inv H4. *)
+    (*   + simpl in *; inv H2; inv H1; dest; repeat split; unfold getLabel; simpl; auto. *)
+    (*   + simpl in *; inv H2; inv H1; dest; repeat split; unfold getLabel; simpl; auto. *)
+    (*   + simpl in *; inv H2; inv H1; dest; repeat split; unfold getLabel; simpl; auto. *)
+    (*   + simpl in *; inv H2; inv H1; dest; repeat split; unfold getLabel; simpl; auto. *)
+    (*   + simpl in *; inv H2; inv H1; dest; repeat split; unfold getLabel; simpl; auto. *)
+    (*   + simpl in *; inv H2; inv H1; dest; repeat split; unfold getLabel; simpl; auto. *)
+    (*   + simpl in *; inv H2; inv H1; dest; repeat split; unfold getLabel; simpl; auto. *)
+    (*   + simpl in *; inv H2; inv H1; dest; repeat split; unfold getLabel; simpl; auto. *)
+    (*   + simpl in *; inv H2; inv H1; dest; repeat split; unfold getLabel; simpl; auto. *)
+    (*   + simpl in *; inv H2; inv H1; dest; repeat split; unfold getLabel; simpl; auto. *)
+    (*   + simpl in *; inv H2; inv H1; dest; repeat split; unfold getLabel; simpl; auto. *)
+    (*   + simpl in *; inv H2; inv H1; dest; repeat split; unfold getLabel; simpl; auto. *)
+    (*   + simpl in *; inv H2; inv H1; dest; repeat split; unfold getLabel; simpl; auto. *)
+    (*   + simpl in *; inv H2; inv H1; dest; repeat split; unfold getLabel; simpl; auto. *)
+    (*   + simpl in *; inv H2; inv H1; dest; repeat split; unfold getLabel; simpl; auto. *)
+    (*   + clear HIn1 HIn2. *)
+    (*     admit. *)
+    (*     (* CommonTactics.dest_in. *) *)
+  Qed.
+  
+End Facts.
+
